# The Natural Numbers

In this chapter natural numbers will by synonym of the positive integers, $\mathbb{P}$. That is, $1, 2, 3, \ldots$, where are one of the most familiar mathematical objects. 

The objective of this chapter is to develop an axiomatic theory of the natural numbers following [@mendelson_introduction_2015, chap. 2].

## Peano systems

::: {#def-peano-system}

A **Peano system** is a triple $(\mathbb{P}, 1, S)$ where $\mathbb{P}$ is a non empty set where $1 \in \mathbb{P}$ and $S$ is a singulary operation on $\mathbb{P}$, $S: \mathbb{P} \longrightarrow \mathbb{P}$, such that the following axioms are satisfied:

i. $1$ is not the successor $S(x)$ of any object $x \in \mathbb{P}$. In symbols, $\forall x(S(x) \neq 1)$ or $1 \not \in \mathscr{R}(S)$.

ii. Different objects in $\mathbb{P}$ have different successors. This can be formulated as follows:

    $$\forall x \forall y (x \neq y \Longrightarrow S(x) \neq (S(y)))$$
    
iii. Principle of Mathematical Induction: Any subset of $\mathbb{P}$ containing $1$ and closed under the successor operation (See @exr-binary-operation 1. and applied for a singulary operation) must be identical to $\mathbb{P}$. This can be formulated as follows:
    
     $$\forall B ((B \subseteq \mathbb{P} \land 1 \in B \land \forall x(x \in B \Longrightarrow S(x) \in B)) \Longrightarrow \mathbb{P} = B)$$

**Note**: In the triple $(\mathbb{P}, 1, S)$ the set $\mathbb{P}$ is called the underlying  set, $S$ the successor operation, and $1$ the distinguished element. The distinguished element $1$ need not have anything to do with the ordinary integer $1$. 

:::

::: {#exm-peano-systems}

1. Let $\mathbb{P}$ be the set of natural numbers. $1$ is to denote the ordinary integer $1$. $S$ is the operation of adding $1$: $S(x) = x + 1$ for all $x \in \mathbb{P}$. This example will be called the standard Peano system. 

   If $x \in \mathbb{P}$ then $x + 1 \neq 1$. Also if $x \neq y$ then $x + 1 \neq y + 1$. Furthermore, let $B \subseteq \mathbb{P}$, $1 \in B$ and if $x \in B$ then $x + 1 \in B$. Therefore $B = \mathbb{P}$.
   
2. Let $\mathbb{P}$ be the set of all integers greater than or equal to $1000$. $1$ is to denote the integer $1000$. $S$ is the operation of adding the ordinary integer $1$. Thus $S(1000) = 1001$, $S(1001) = 1002$ and so on.

3. Let $\mathbb{P}$ be the set of negative integers. $1$ is to denote the integer $-1$ and $S$ is the operation of subtracting $1$.  Thus $S(-1) = -2$, $S(-2) = -3$ and so on.  

4. Let $\mathbb{P}$ be the set of even positive integers. Let $1$ denote the integer $2$. $S$ is to be the operation of adding $2$. Thus, $S(2) = 4$, $S(4)$ and so on.

:::

::: {#thm-x-different-1-is-a-successor}

Every element different from $1$ is a successor. This can be formulated as:

$$\forall x (x = 1 \lor \exists y (x = S(y)))$$

:::

::: {.proof}

Let $B = \{ x \in \mathbb{P}: x = 1 \lor \exists y (x = S(y)) \}$. Then we must show that $B = \mathbb{P}$.

We have that $1 \in B$. Now assume $x \in B$ then $x \in \mathbb{P}$. Because $S: \mathbb{P} \longrightarrow \mathbb{P}$ then $S(x) \in \mathbb{P}$ where $S(x) \neq 1$. So if $x = y$ it exists some $y$ such that $S(x) = S(y)$. Therefore $S(x) \in B$ which means that $B = \mathbb{P}$ by @def-peano-system iii.

:::

::: {#thm-no-object-is-its-own-successor}

No object is its own successor, that is, $\forall x (S(x) \neq x)$.

:::

::: {.proof}

Let $B = \{ x \in \mathbb{P}: S(x) \neq x \}$. Then we must show that $B = \mathbb{P}$.

We have that $1 \in B$ because $S(1) \neq 1$ by @def-peano-system i. Also let $x \in B$ so $x \in \mathbb{P}$ and $S(x) \neq x$. Furthermore $S(x) \in \mathbb{P}$ because $S: \mathbb{P} \longrightarrow \mathbb{P}$. By @def-peano-system ii $S(S(x)) \neq S(x)$ so $S(x) \in B$. Finally by @def-peano-system iii $B = \mathbb{P}$. 

:::

::: {#exr-peano-systems}

1. Prove that every object different from $1$ is the successor for a unique object, that is, 

   $$\forall x (x = 1 \lor \exists !y (x = S(y)))$$

2. Prove $\forall x (x = 1 \lor x = S(1) \lor \exists y (x = S(S(y))))$

3. Determine whether or not the following structures $(\mathbb{P}, S, 1)$ are Peano Systems:

    a. $\mathbb{P}$ is a set of all integers greater than $9$. $1$ stands for the integer $10$. $S(u) = u + 1$ for any $u \in P$, that is $S$ is the operation of adding the ordinary integer $1$.
    
    b. $\mathbb{P}$ is a set of all integers. $1$ stands for the ordinary integer $1$. $S(u) = u + 1$ for any $u \in P$.
    
    c. $\mathbb{P}$ is the set of all integers. $1$ stands for the ordinary integer $0$ and $S(u)$ is defined us:
        
       $$S(u) = \begin{cases}
                 1      & \text{if} u = 0 \\
                 -u     & \text{if} u > 0 \\
                 -(u-1) & \text{if} u < 0
                \end{cases}$$
                
       ![$S(u)$ for $\mathbb{Z}$](images/fig-successor-integers.png){#fig-successor-integers fig-align="center" width=40%}

    d. $\mathbb{P}$ is the set of rational numbers of the form $\frac{1}{2^n}$ where $n$ is a non negative integer. $1$ stands for the integer $1$. Also $S(u) = \frac{1}{2}u$ for all $u \in \mathbb{P}$.
    
    e. $\mathbb{P} = \{ 1, 2, 3, 4 \}$. $1$ stands for the integer $1$. Also $S(1) = 2$, $S(2) = 3$, $S(3) = 4$ and $S(4) = 1$.

    f. $\mathbb{P} = \{ 1, 2, 3, \ldots \} \cup \{ 1\#, 2\#, 3\#, \ldots \}$ where $1\#$, $2\#$, $3\#$, $\ldots$ are pairwase distinct new objects different from the natural numbers. Let $1$ denote the integer 1. Let $S(n) = n + 1$ for any positive integer $n$ and let $S(n\#) = (n + 1)\#$ for any positive integer $n$. Thus, $S(1) = 2$, $S(2) = 3$, $\ldots$, and $S(1\#) = 2\#$, $S(2\#) = 3\#$, $\ldots$

:::

::: {#sol-peano-systems}

1. By @thm-no-object-is-its-own-successor we have that:

   $$\forall x (x = 1 \lor \exists y (x = S(y)))$$
   Now assume that $x = S(y)$ and $x = S(w)$ so $S(y) = S(w)$. By @def-peano-system ii $y = w$. Therefore:
   
   $$\forall x (x = 1 \lor \exists !y (x = S(y)))$$

2. We have that $1 \in B$. Now assume $y \in B$ then $y \in \mathbb{P}$. Because $S: \mathbb{P} \longrightarrow \mathbb{P}$ then $S(y) \in \mathbb{P}$ where $S(y) \neq 1$. Furthermore by @def-peano-system ii $S(S(y)) \neq S(1)$. 

   If $y = 1$ then $S(1) \neq 1$ and by @thm-x-different-1-is-a-successor $x = S(1)$.
   
   Also if $S(S(y))$ and $y \neq 1$ by @thm-x-different-1-is-a-successor $\exists y (x = S(S(y)))$. Therefore:
   
   $$\forall x (x = 1 \lor x = S(1) \lor \exists y (x = S(S(y))))$$

3. In each $(\mathbb{P}, S, 1)$ we have the following results

    a. Because $\mathbb{P} = \{ u : u > 9 \land u \text{ is an integer} \}$. 
   
        - First $S(u) = u + 1$ where $u \in \mathbb{P}$ then $S(u) \neq 10$. Because if $u + 1 = 10$ then $u = 9$ but $9 \not \in \mathbb{P}$.
   
        - Also let $S(u) = S(v)$ so $u + 1 = v + 1$ which means that $u = v$.
      
        - Finally let $10 \in B \subseteq \mathbb{P}$ and if $u \in B$ then $u + 1 \in B$. 
      
            - Let $v \in \mathbb{P}$ so we need to prove that $v \in B$. Define $A = \{ x \in \mathbb{P} \mid 10 \leq x \leq v \}$ and let $B \cap A$
         
                - First, we have that $B \cap A \subseteq A$ so by @thm-finite-set b $B \cap A$ must be finite. Furthermore $B \cap A \neq \emptyset$ because $10 \in B$ and $10 \in A$.
         
                - Second, because $B \cap A$ is finite and $B \cap A \neq \emptyset$ it must have a greatest element $k$. **Pending reference Appendix D** 
         
                    - If $k = v$ then $v \in B$
            
                    - If $k < v$ and because $k \in B \cap A$ then $k \in B$. Because of the properties of $B$ then $k + 1 \in B$. Also this means that $10 \leq k + 1 \leq v$ so $k + 1 \in A$ but this will mean that $k + 1 \in B \cap A$. However $k + 1 > k$ so $k$ will not be the greatest element. Because we arrive to a contradiction we discard that $k < v$. 

    b. The proof is similar to @sol-peano-systems 3 a but with $1$ instead of $10$ and $\mathbb{P} = \{ u : u > 0 \land x \text{ is an integer} \}$
    
    c. Let $\mathbb{P} = \mathbb{Z}$
    
        - Because $S(u) = 1, S(u) = -u < 0$ or $S(u) = -(u - 1) > 1$ then $S(u) \neq 0$
    
        - Also if $S(u) = S(v)$ then $1 = 1$ so $u = v = 0$, $-u = -v$ so $u = v$ or $-(u - 1) = -(v - 1)$ so $u = v$.
       
        - Finally let $0 \in B \subseteq \mathbb{P}$ and if $u \in B$ then $S(u) \in B$. 
        
           - Let $v \in \mathbb{P}$ so we need to prove that $v \in B$. Lets define the set $A$ in the following way:
        
             $$A = \begin{cases}
                    \{x \in \mathbb{P} \mid -(v - 1) \leq x \leq v \} & \text{ if } v > 0 \\
                    \{x \in \mathbb{P} \mid v \leq x \leq -v \} & \text{ if } v \leq 0
                   \end{cases}$$

              - First, we have that $B \cap A \subseteq A$ so by @thm-finite-set b $B \cap A$ must be finite. Furthermore $B \cap A \neq \emptyset$ because $0 \in B$ and $0 \in A$.
              
              - Second, because $B \cap A$ is finite and $B \cap A \neq \emptyset$ it must have a greatest element $k$ and a least element $l$ **Pending specify that you can extend reference Appendix D**.
              
                 - If $k = v > 0$ or $l = v \leq 0$ then $v \in B$
                 
                 - If $k < v$ and $v > 0$ because $k \in B \cap A$ then $k \in B$. Also because of the properties of $B$ then $S(k) \in B$. 
                 
                    - If $k = 0$ then $S(k) = 1 \in B$ and $-(v - 1) \leq 1 \leq v$ so $1 \in A$ but this will mean that $1 \in B \cap A$. However $1 > 0$ so $0$ will not be the greatest element. Because we arrive to a contradiction we discard that $k < v$ when $k = 0$.
                    
                    - If $k > 0$ then $S(k) = -k \in B$ and $S(-k) = -(-k - 1) = k + 1 \in B$. Therefore $-(v - 1) \leq k + 1 \leq v$ so $k+1 \in A$ but this will mean that $k+1 \in B \cap A$. However $k+1 > k$ so $k$ will not be the greatest element. Because we arrive to a contradiction we discard that $k < v$ when $k > 0$.
                    - If $k < 0$ then we discard this case because $0 \in B \cap A$ so if $k < 0$ it can not be the greatest element. 

                 - If $v < l$ and $v \leq 0$ because $l \in B \cap A$ then $l \in B$. Also because of the properties of $B$ then $S(l) \in B$.

                    - If $l = 0$ then $S(l) = 1 \in B$ and $S(1) = -1$. Therefore $v \leq -1 \leq -v$ so $-1 \in A$ but this will mean that $-1 \in B \cap A$. However $-1 < 0$ so $0$ will not be the least element. Because we arrive to a contradiction we discard that $v < l$ when $l = 0$.

                    - If $l > 0$ then we discard this case because $0 \in B \cap A$ so if $l > 0$ it can not be the least element.

                    - If $l < 0$ then $S(l) = -(l - 1) = -l + 1 \in B$ and $S(-l + 1) = l - 1 \in B$. Therefore $v \leq l - 1 \leq -v$ so $l - 1 \in A$ but this will mean that $l - 1 \in B \cap A$. However $l - 1 < l$ so $l$ will not be the least element. Because we arrive to a contradiction we discard that $v < l$ when $l < 0$.

    d. Let $\mathbb{P} = \{ u \mid u = \frac{1}{2^n} \land n \in \mathbb{Z}_{\geq 0} \}$
    
        - First $S(u) = \frac{1}{2}u$ where $u = \frac{1}{2^n}$ then $S(u) \neq 1$. Because if $\frac{1}{2}u = 1$ then $u = 2$ but $u = \frac{1}{2^n}$. So $u = 2$ will imply $\log_2 1 = n + 1$ but this is not true because $n \neq -1$.
        
        - Also let $S(u) = S(v)$ so $\frac{1}{2}u = \frac{1}{2}v$ which means that $u = v$. 
        
        - Finally let $1 \in B \subseteq \mathbb{P}$ and if $u \in B$ then $S(u) \in B$. 
      
            - Let $v \in \mathbb{P}$ so we need to prove that $v \in B$. Define $A = \{ x \in \mathbb{P} \mid v \leq x \leq 1 \}$ and let $B \cap A$
            
                - First, we have that $B \cap A \subseteq A$ so by @thm-finite-set b $B \cap A$ must be finite. Furthermore $B \cap A \neq \emptyset$ because $1 \in B$ and $1 \in A$.

                - Second, because $B \cap A$ is finite and $B \cap A \neq \emptyset$ it must have a least element $l$. **Pending specify that you can extend reference Appendix D** 
         
                    - If $l = v$ then $v \in B$
            
                    - If $v < l$ and because $l \in B \cap A$ then $l \in B$. Because of the properties of $B$ then $S(l) = \frac{1}{2}l \in B$. Also this means that $v \leq \frac{1}{2}l \leq 1$ so $\frac{1}{2}l \in A$ but this will mean that $\frac{1}{2}l \in B \cap A$. However $\frac{1}{2}l < l$ so $l$ will not be the least element. Because we arrive to a contradiction we discard that $v < l$.  

    d. Because $\mathbb{P} = \{ 1, 2, 3, 4 \}$ and $S(1) = 2$, $S(2) = 3$, $S(3) = 4$, $S(4) = 1$ we have that this structure is not a peano system because:
    
        - $S(4) = 1$ 

    f. Because $\mathbb{P} = \{ 1, 2, 3, \ldots \} \cup \{ 1\#, 2\#, 3\#, \ldots \}$, $S(n) = n + 1$ and $S(n\#) = (n + 1)\#$ we have that this structure is not a peano system because:
    
        - Assume $1 \in B$ where $B = \{ 1, 2, 3, \ldots \} \subseteq \mathbb{P}$ and if $u \in B$ then $S(u) \in B$.
        
           - By @exr-peano-systems 3 b $B = \{ 1, 2, 3, \ldots \}$ where $B \neq \mathbb{P}$. 
:::

## Diagramatic interpretation of peano system axioms

Following [@enderton_elements_2009, p. 70] we can specify different interpretations of the axioms presented in @def-peano-system. 

In the case of the first axiom @def-peano-system i if $\mathbb{P} = \{ 1, 2, 3 \}$, $S(1) = 2$, $S(2) = 3$ and $S(3) = 1$ a representation of the violation of this axiom is represented in @fig-peano-axiom-1-violation:

![Violation of the first peano axiom](images/fig-peano-axiom-1-violation.png){#fig-peano-axiom-1-violation fig-align="center" width=20%}

The axiom pointed out in @def-peano-system i avoid that you can return to the origin $1$ using the successor function $S$.

In the case of the second axiom @def-peano-system ii if $\mathbb{P} = \{ 1, 2, 3 \}$, $S(1) = 2$, $S(2) = 3$ and $S(3) = 2$ a representation of the violation of this axiom is represented in @fig-peano-axiom-2-violation:

![Violation of the second peano axiom](images/fig-peano-axiom-2-violation.png){#fig-peano-axiom-2-violation fig-align="center" width=20%}

The axiom pointed out in @def-peano-system ii avoid that you can have loops using the successor function $S$.

In the case of the third axiom @def-peano-system iii if $\mathbb{P} = \{ 1, 2, 3, \ldots \} \cup \{ \omega \}$ where $\{ 1, 2, 3, \ldots \} \cap \{ \omega \} = \emptyset$ , $S(1) = 2$, $S(2) = 3$, $\ldots$, $\omega = S(\omega)$ a representation of the violation of this axiom is represented in @fig-peano-axiom-3-violation:

![Violation of the third peano axiom](images/fig-peano-axiom-3-violation.png){#fig-peano-axiom-3-violation fig-align="center" width=30%}

The axiom pointed out in @def-peano-system iii avoid that you can not reach an element in $\mathbb{P}$ using the successor function $S$ and beginning at the origin $1$.

## The iteration theorem

Any arithmetical notions such as $+$ and $\times$ are not mentioned in @def-peano-system. These notions will be defined by induction. The idea of the definition by induction is different from that of proof by mathematical induction pointed out in @def-peano-system iii.

When we define a function $f$ by induction, we first specify $f(1)$ and then indicate a rule for obtaining $f(S(x))$ from the previous value $f(x)$. This determines a unique function $f$ defined on $\mathbb{P}$.

::: {#thm-iteration-theorem}

## Iteration theorem[^chapter_2-1]

Consider any peano system $(\mathbb{P}, S, 1)$. Let $W$ be an arbitrary set, let $c$ be a fixed element of $W$, and let $g$ be a singulary operation on $W$, that is $g: W \longrightarrow W$. Then, there is a unique function $F: \mathbb{P} \longrightarrow W$ such that:

a. $F(1) = c$
b. $F(S(x)) = g(F(x))$ for all $x \in \mathbb{P}$

:::

[^chapter_2-1]: Also known as the recursion theorem (See [@enderton_elements_2009, pp. 73-74]) where it can be found in [@dedekind_essays_1963, pp. 85-86]

::: {.proof}

- Existence of a suitable function $F$

  Take any $n \in \mathbb{P}$. A function $f: A \longrightarrow W$ is said to be $n$-admissible if and only if:
  
    i. $A \subseteq \mathbb{P}$
  
    ii. $1 \in A$
    
    iii. $n \in A$
    
    iv. $\forall u (S(u) \in A \Longrightarrow u \in A)$
    
    v. $f(1) = c$
    
    vi. $\forall u (S(u) \in A \Longrightarrow f(S(u)) = g(f(u)))$
    
        a. If $f$ is $S(n)$-admissible, then $f$ is $n$-admissible
        
           If conditions i, ii and iv-vi are fulfill for $S(n)$ they are also fulfill for $n$. The only condition that we need to check is iii, that is $n \in A$. Because $f$ is $S(n)$-admissible by iii $S(n) \in A$. Therefore by iv $n \in A$.
           
        b. For any $n \in \mathbb{P}$ there exists at least one $n$-admissible function.
        
           We shall prove this by mathematical induction using @def-peano-system i. Let $B$ be the set of all members $n \in P$  for which there exists at least one $n$-admissible function.
           
           We must show that $B = \mathbb{P}$. First, lets build a $1$-admissible function. Let $A = \{ 1 \}$ then $\{ 1 \} \subseteq \mathbb{P}$, $1 \in \{ 1 \}$, $S(1) \neq \{ 1 \}$ and $f(1) = c$. Therefore $f: \{ 1 \} \longrightarrow W$ is $1$-admissible.
           
           Second, assume $n \in B$. Then by assumption there is some $n$-admissible function $f$ such that $f: A \longrightarrow W$.
           
           Third, define a function $f^*$ such that for any $x \in A$ $f^*(x) = f(x)$ and if $S(n) \not \in A$ let $f^*(S(n)) = g(f(n))$. Note that if $S(n) \in A$ then by vi $f(S(u)) = g(f(u))$. Therefore, $f^*: A^* \longrightarrow W$ such that $A^* = A \cup \{ S(n) \}$ where $A \subseteq A^*$. So $A^* \subseteq \mathbb{P}$, $1 \in A^*$, $n \in A^*$, if $S(n) \not \in A$ then $S(n) \in A^*$ then $n \in A^*$, $f^*(1) = f(1) = c$ and if $S(n) \not \in A$ then $S(n) \in A^*$ implies that $f^*(S(n)) = g(f(n))$. This means that $f^*$ is $S(n)$-admissible.
           
           Thus, $S(n) \in B$. We have shown that if $n \in B$ then $S(n) \in B$. By @def-peano-system iii $B = \mathbb{P}$.

        c. If $f$ is $n$-admissible and $h$ is $n$-admissible then $f(n) = h(n)$.
        
           We shall prove this by mathematical induction. Let $Y = \{ n \in \mathbb{P} \mid (\forall f) (\forall g) (((f \text{ is } n\text{-admissible} \land (g \text{ is } n\text{-admissible} )) \Longrightarrow f(n) = g(n)) \}$. We must show that $Y = \mathbb{P}$ using @def-peano-system iii.
           
           First, $1 \in Y$ because $1 \in \mathbb{P}$ and if $f$ and $g$ are $1$-admissible then $f(1) = c = g(1)$.
           
           Second, assume $n \in Y$.
           
           Third, let $f$ and $h$ be $S(n)$-admissible. Then by a. $f$ and $h$ are $n$-admissible. Because $n \in Y$ then $f(n) = h(n)$. By vi. $f(S(n)) = g(f(n))$ but $f(n) = h(n)$ so $f(S(n)) = g(h(n))$. Again by vi. $f(S(n)) = h(S(n))$.Therefore $S(n) \in Y$ so $Y = \mathbb{P}$   
           
        d. For any $n \in \mathbb{P}$ by b. it  exists an $n$-admissible function $f$. 
           
           Let us define $F(n) = f(n)$. By c. the value of $F(n)$ does not depend upon the particular choice of the $n$-admissible function $f$.
           
           Because we choose any $n \in \mathbb{P}$ then $\mathscr{D}(F) = \mathbb{P}$. Also, $F(1) = f(1)$ for some $1$-admissible function $f$. But, $f(1) = c$. Hence we have that $F(1) = c$.
           
           In addition, $F(S(n)) = f(S(n))$ for some $S(n)$-admissible function $f$. By a. $f$ is also $n$-admissible where $F(n) = f(n)$. Also since $f$ is $S(n)$-admissible, $f(S(n)) = g(f(n))$ we have that $F(S(n)) = g(F(n))$.
           
           Therefore conditions a. and b. in @thm-iteration-theorem are satisfied by $F$.
           
           We must still show that the range of $F$ is included in $W$. Because for any $n \in \mathbb{P}$, $F(n) = f(n)$ for some $n$-admissible function $f$. Since $\mathscr{R}(f) \subseteq W$, it follows that $F(n) \in W$ for any $n \in \mathbb{P}$.

- Uniqueness of $F$

  Assume $F_1$ and $F_2$ are functions from $\mathbb{P}$ into $W$ satisfying conditions a. and b. in @thm-iteration-theorem.
  
  Let $K = \{ n \in \mathbb{P} \mid \land F_1(n) = F_2(n) \}$.
  
  First, $1 \in K$ because $F_1(1) = c = F_2(1)$.
  
  Second, assume $n \in K$ so $F_1(n) = F_2(n)$.
  
  Third, let $F_1(S(n))$ then $F_1(S(n)) = g(F_1(n))$. Therefore $g(F_1(n)) = g(F_2(n))$ which means that $g(F_2(n)) = F_2(S(n))$. So $F_1(S(n)) = F_2(S(n))$. 
  
  By @def-peano-system iii $K = \mathbb{P}$ so for all $n \in \mathbb{P}$ we have that $F_1(S(n)) = F_2(S(n))$. Also $\mathscr{D}(F_1) = \mathscr{D}(F_2)$ so by @exr-function 3 $F_1 = F_2$. 

:::